isabelle/CVM_clean/CVM_Algo_Proof.thy
@@ -1,22 +1,25 @@
 theory CVM_Algo_Proof
-  imports
-    CVM_Algo
+
+imports
+  CVM_Algo
+
 begin
 
 locale cvm_algo_proof = cvm_algo +
-  assumes "f \<in> {1/2..<1}"
+  assumes f : \<open>1 / 2 \<le> f\<close> \<open>f < 1\<close>
 begin                       
 
 (* Copied as-is for Lemma 2 *)
 context
-  fixes \<phi> :: "real \<Rightarrow> bool \<Rightarrow> real"
-  assumes pos :"\<And>x b. x \<in> {0<..1} \<Longrightarrow> \<phi> x b \<ge> 0"
-  assumes c1: \<open>\<And>\<alpha> x.
-    \<alpha> \<in> {0<..<1} \<Longrightarrow> x \<in> {0<..1} \<Longrightarrow>
-    (1 - \<alpha>) * \<phi> x False + \<alpha> * \<phi> x True \<le> \<phi> (x / \<alpha>) True \<close>
-  assumes c2: "\<And>x y.
-    0 < x \<Longrightarrow> x \<le> y \<Longrightarrow> y \<le> 1 \<Longrightarrow>
-    \<phi> x False \<le> \<phi> y False"
+  fixes \<phi> :: \<open>real \<Rightarrow> bool \<Rightarrow> real\<close>
+  assumes phi : 
+    \<open>\<And> x b. \<lbrakk>0 < x; x \<le> 1\<rbrakk> \<Longrightarrow> \<phi> x b \<ge> 0\<close> and
+    \<open>\<And> \<alpha> x.
+      \<lbrakk>0 < \<alpha>; \<alpha> < 1; 0 < x; x \<le> 1\<rbrakk> \<Longrightarrow>
+      (1 - \<alpha>) * \<phi> x False + \<alpha> * \<phi> x True \<le> \<phi> (x / \<alpha>) True \<close> and
+    \<open>\<And> x y.
+      \<lbrakk>0 < x; x \<le> y; y \<le> 1\<rbrakk> \<Longrightarrow>
+      \<phi> x False \<le> \<phi> y False\<close>
 begin
 
 abbreviation (input)
@@ -31,83 +34,102 @@ abbreviation (input)
     state_chi st \<subseteq> U
 *)
 
-lemma expectation_step1:
-  assumes U: "finite U"
-  assumes "\<And>S.
+lemma step_1_preserves_expectation_le :
+  assumes
+    \<open>finite U\<close>
+    \<open>\<And> S.
       S \<subseteq> U \<Longrightarrow>
-      measure_pmf.expectation stp (prod aux S) \<le> (\<phi> 1 True) ^ card S"
-  assumes "S \<subseteq> insert x U"
-  shows "
-    measure_pmf.expectation (stp \<bind> step1 x) (prod aux S)
-      \<le> (\<phi> 1 True) ^ card S"
-  sorry
+      measure_pmf.expectation state (prod aux S) \<le> (\<phi> 1 True) ^ card S\<close>
+    \<open>S \<subseteq> insert x U\<close>
+  shows
+    \<open>measure_pmf.expectation (state \<bind> step_1 x) (prod aux S)
+    \<le> (\<phi> 1 True) ^ card S\<close>
+proof - 
+  show ?thesis sorry
+qed
 
-lemma expectation_step2:
-  assumes U: "finite U"
-  assumes "measure_pmf.expectation stp (prod aux S) \<le> (\<phi> 1 True) ^ card S"
-  assumes "S \<subseteq> U"
-  shows "
-    measure_pmf.expectation (stp \<bind> step2) (prod aux S) \<le> (\<phi> 1 True) ^ card S"
-  sorry
+lemma step_2_preserves_expectation_le :
+  assumes
+    \<open>finite U\<close>
+    \<open>measure_pmf.expectation state (prod aux S) \<le> (\<phi> 1 True) ^ card S\<close>
+    \<open>S \<subseteq> U\<close>
+  shows
+    \<open>measure_pmf.expectation (state \<bind> step_2) (prod aux S)
+    \<le> (\<phi> 1 True) ^ card S\<close>
+proof - 
+  show ?thesis sorry
+qed
 
-lemma expectation_cvm_step:
-  assumes U: "finite U"
-  assumes "\<And>S.
+lemma step_preserves_expectation_le :
+  assumes
+    \<open>finite U\<close>
+    \<open>\<And> S.
       S \<subseteq> U \<Longrightarrow>
-      measure_pmf.expectation stp (prod aux S) \<le> (\<phi> 1 True) ^ card S"
-  assumes "S \<subseteq> insert x U"
-  shows "
-    measure_pmf.expectation (stp \<bind> cvm_step x) (prod aux S) \<le> (\<phi> 1 True) ^ card S"
-  sorry
+      measure_pmf.expectation state (prod aux S) \<le> (\<phi> 1 True) ^ card S\<close>
+    \<open>S \<subseteq> insert x U\<close>
+  shows
+    \<open>measure_pmf.expectation (state \<bind> cvm_step x) (prod aux S)
+    \<le> (\<phi> 1 True) ^ card S\<close>
+proof - 
+  show ?thesis sorry
+qed
 
 lemma expectation_cvm:
-  assumes U: "finite U"
-  assumes "\<And>S.
+  assumes
+    \<open>finite U\<close>
+    \<open>\<And>S.
       S \<subseteq> U \<Longrightarrow>
-      measure_pmf.expectation stp (prod aux S) \<le> (\<phi> 1 True) ^ card S"
-  assumes "S \<subseteq> set xs \<union> U"
-  shows "
-    measure_pmf.expectation (stp \<bind> cvm xs) (prod aux S) \<le> (\<phi> 1 True) ^ card S"
-  sorry
+      measure_pmf.expectation state (prod aux S) \<le> (\<phi> 1 True) ^ card S\<close>
+  assumes \<open>S \<subseteq> set xs \<union> U\<close>
+  shows
+    \<open>measure_pmf.expectation (state \<bind> run_steps xs) (prod aux S)
+    \<le> (\<phi> 1 True) ^ card S\<close>
+proof - 
+  show ?thesis sorry
+qed
 
 (* Run some prefix of the elements + one more *)
-lemma expectation_cvm_step1:
-  assumes U: "finite U"
-  assumes "\<And>S.
+lemma run_steps_then_step_1_preserves_expectation_le :
+  assumes
+    \<open>finite U\<close>
+    \<open>\<And>S.
       S \<subseteq> U \<Longrightarrow>
-      measure_pmf.expectation stp (prod aux S) \<le> (\<phi> 1 True) ^ card S"
-  assumes "S \<subseteq> insert x (set xs \<union> U)"
-  shows "
-    measure_pmf.expectation (stp \<bind> cvm xs \<bind> step1 x) (prod aux S) \<le> (\<phi> 1 True) ^ card S"
-  sorry
+      measure_pmf.expectation stp (prod aux S) \<le> (\<phi> 1 True) ^ card S\<close>
+    \<open>S \<subseteq> insert x (set xs \<union> U)\<close>
+  shows
+    \<open>measure_pmf.expectation (stp \<bind> run_steps xs \<bind> step_1 x) (prod aux S)
+    \<le> (\<phi> 1 True) ^ card S\<close>
+proof -
+  show ?thesis sorry
+qed
 
 end
 
-
 context
-  fixes q :: real
-  fixes h :: "real \<Rightarrow> real"
-  assumes "q \<in> {0<..1}"
-  assumes "concave_on {0..1/q} h"
-  assumes "\<And>x. x \<in> {0..1/q} \<Longrightarrow> h x \<ge> 0"
+  fixes q :: real and h :: \<open>real \<Rightarrow> real\<close>
+  assumes
+    \<open>0 < q\<close> \<open>q \<le> 1\<close> and
+    \<open>concave_on {0 .. 1 / q} h\<close> and
+    \<open>\<And> x. \<lbrakk>1 \<le> x; x * q \<le> 1\<rbrakk> \<Longrightarrow> h x \<ge> 0\<close>
 begin
 
 abbreviation (input)
-  \<open>aux2 \<equiv> \<lambda> x state. (
-    let p = f ^ (state_k state) in
-    of_bool (p > q) * h ((1 / p) * indicat_real (state_chi state) x)
-  )\<close>
+  \<open>aux' \<equiv> \<lambda> x state. (
+    let p = f ^ (state_k state)
+    in of_bool (p > q) * h ((1 / p) * indicat_real (state_chi state) x))\<close>
 
 (* Lemma 3 *)
-lemma expectation_cvm':
-  assumes U: "finite U"
-  assumes "\<And>S.
+lemma expectation_cvm' :
+  assumes U: \<open>finite U\<close>
+  assumes \<open>\<And> S.
       S \<subseteq> U \<Longrightarrow>
-      measure_pmf.expectation stp (prod aux2 S) \<le> (h 1) ^ card S"
-  assumes "S \<subseteq> set xs \<union> U"
-  shows "
-    measure_pmf.expectation (stp \<bind> cvm xs) (prod aux2 S) \<le> (h 1) ^ card S"
-  sorry
+      measure_pmf.expectation stp (prod aux' S) \<le> (h 1) ^ card S\<close>
+  assumes \<open>S \<subseteq> set xs \<union> U\<close>
+  shows
+    \<open>measure_pmf.expectation (stp \<bind> cvm xs) (prod aux2 S) \<le> (h 1) ^ card S\<close>
+proof -
+  show ?thesis sorry
+qed
 
 end
 
